theories/Handlers/Deterministic.v
@@ -1,5 +1,5 @@
 (* SLOT, a formally verified model checker
-   Copyright (C) 2019-2023  k32
+   Copyright (C) 2019-2024  k32
 
    This program is free software: you can redistribute it and/or modify
    it under the terms of the GNU General Public License as published by
@@ -29,9 +29,7 @@ From LibTx Require Import
      Storage.Classes.
 
 From SLOT Require Import
-     Foundations
-     Commutativity
-     Tactics.
+     Foundations.
 
 From Hammer Require Import
      Tactics.
